feat: export Lean to HTML (#537)
This PR adds two executables:

* verso-literate: this uses elaborated Verso moduledocs and docstrings to create a richer representation of a Lean module than the prior literate module support, and with less overhead from heuristic Markdown processing.

* verso-html: this takes the results of verso-literate and produces an HTML rendering of source code. Perhaps ironically, this fails on Verso documents due to differences in the parser's output, but it can render the rest of Verso's source without issue.

It also adds the ability for the blog genre and the manual genre to include text using verso-literate, so they can load arbitrary Lean files with Verso moduledocs and treat them as content.

src/multi-verso/MultiVerso.lean
@@ -3,17 +3,22 @@ Copyright (c) 2023-2025 Lean FRO LLC. All rights reserved.
 Released under Apache 2.0 license as described in the file LICENSE.
 Author: David Thrane Christiansen
 -/
+module
 
-import Lean.Data.Json
+public import Lean.Data.Json
 
 import Std.Data.TreeMap
 import Std.Data.HashSet
+import Std.Time.Zoned
+import Std.Time.Format
 
-import MultiVerso.InternalId
-import MultiVerso.Link
+public import MultiVerso.InternalId
+public import MultiVerso.Link
 import MultiVerso.Manifest
 import MultiVerso.Path
 import MultiVerso.Slug
+
+set_option doc.verso true
 
 open Std
 open Lean
@@ -25,7 +30,7 @@ namespace Verso.Multi
 /--
 A documented object, described in specific locations in the document.
 -/
-structure Object where
+public structure Object where
   /--
   The canonical string name used to construct a cross-reference to this object, also from external
   sites. Should be stable over time.
@@ -38,7 +43,7 @@ structure Object where
 deriving Inhabited
 
 open Format in
-instance : Repr Object where
+public instance : Repr Object where
   reprPrec v _ :=
     let {canonicalName, data, ids} := v
     nest 2 <| group <| line.joinSep [
@@ -49,7 +54,7 @@ instance : Repr Object where
       text "}"
     ]
 
-instance : BEq Object where
+public instance : BEq Object where
   beq
     | {canonicalName := n1, data := d1, ids := i1}, {canonicalName := n2, data := d2, ids := i2} =>
       n1 == n2 &&
@@ -57,30 +62,34 @@ instance : BEq Object where
       i1.size == i2.size && i1.fold (init := true) (fun soFar v => soFar && i2.contains v)
 
 /--
-Registers the fact that the provided `id` refers to the object.
+Registers the fact that the provided {name}`id` refers to the object.
 -/
-def Object.addId (id : InternalId) (object : Object) : Object :=
+public def Object.addId (id : InternalId) (object : Object) : Object :=
   {object with ids := object.ids.insert id}
 
 /--
-Sets the `data` field of the object, replacing existing data.
+Sets the {name (full := Object.data)}`data` field of the object, replacing existing data.
 -/
-def Object.setData (data : Json) (object : Object) : Object :=
-  {object with data := data}
+public def Object.setData (data : Json) (object : Object) : Object :=
+  { object with data := data }
 
 /--
-Modifies the `data` field of the object.
+Modifies the {name (full := Object.data)}`data` field of the object.
 -/
-def Object.modifyData (f : Json → Json) (object : Object) : Object :=
+public def Object.modifyData (f : Json → Json) (object : Object) : Object :=
   {object with data := f object.data}
 
 /--
 A particular category of documentable objects.
 -/
-structure Domain where
+public structure Domain where
   /-- The objects in the domain, categorized by their canonical names. -/
   objects : TreeMap String Object compare := {}
-  /-- The objects in the domain, categorized by their internal IDs. -/
+  /--
+  The objects in the domain, categorized by their internal IDs. The values in the map are all
+  canonical names for an object with the given ID. In most use cases, without aliasing, the set will
+  be a singleton.
+  -/
   objectsById : TreeMap InternalId (HashSet String) := {}
   /--
   An explanatory title for clients of the domain.
@@ -109,14 +118,21 @@ private unsafe def Domain.fastBeq (x y : Domain) : Bool :=
 Compares two domains for equality.
 -/
 @[implemented_by Domain.fastBeq]
-def Domain.beq (x y : Domain) : Bool := Domain.structBeq x y
+private def Domain.beq (x y : Domain) : Bool := Domain.structBeq x y
 
-instance : BEq Domain := ⟨Domain.beq⟩
+public instance : BEq Domain where
+  beq := private Domain.beq
 
 /--
-Registers the fact that the given ID refers to the object with the given canonical name.
+Returns the canonical names used in {name}`domain`.
 -/
-def Domain.insertId (canonicalName : String) (id : InternalId) (domain : Domain) : Domain :=
+public def Domain.canonicalNames (domain : Domain) : Array String :=
+  domain.objects.keysArray
+
+/--
+Registers the fact that the unique ID {name}`id` refers to the object with the given canonical name.
+-/
+public def Domain.insertId (canonicalName : String) (id : InternalId) (domain : Domain) : Domain :=
   { domain with
     objects :=
       domain.objects.alter canonicalName fun
@@ -129,29 +145,42 @@ def Domain.insertId (canonicalName : String) (id : InternalId) (domain : Domain)
   }
 
 /--
-Sets the `data` field of the object with the given canonical name, replacing existing data.
+Sets the {name (full := Object.data)}`data` field of the object with the given canonical name, replacing existing data.
 -/
-def Domain.setData  (canonicalName : String) (data : Json) (domain : Domain) : Domain :=
+public def Domain.setData  (canonicalName : String) (data : Json) (domain : Domain) : Domain :=
   { domain with objects := domain.objects.alter canonicalName (·.getD {canonicalName} |>.setData data) }
 
 /--
-Modifies the `data` field of the object with the given canonical name.
+Modifies the {name (full := Object.data)}`data` field of the object with the given canonical name.
 -/
-def Domain.modifyData  (canonicalName : String) (f : Json → Json) (domain : Domain) : Domain :=
+public def Domain.modifyData  (canonicalName : String) (f : Json → Json) (domain : Domain) : Domain :=
   { domain with objects := domain.objects.alter canonicalName (·.getD {canonicalName} |>.modifyData f) }
 
 /--
-Returns the object with the given canonical name, or `none` if there is no such object.
+Returns the object with the given canonical name, or {name}`none` if there is no such object.
 -/
-def Domain.get? (canonicalName : String) (domain : Domain) : Option Object :=
+public def Domain.get? (canonicalName : String) (domain : Domain) : Option Object :=
   domain.objects[canonicalName]?
+
+public instance : GetElem? Domain String Object (fun dom x => dom.get? x |>.isSome) where
+  getElem dom x valid :=
+    match h : dom.get? x with
+    | none => False.elim <| by simp_all
+    | some v => v
+  getElem? dom x := dom.get? x
+
+/--
+Returns {name}`true` if the domain contains an object with the given canonical name, or {name}`false` otherwise.
+-/
+public def Domain.contains (canonicalName : String) (domain : Domain) : Bool :=
+  domain.objects.contains canonicalName
 
 /--
 Generates the public cross-reference file for a set of domains.
 
-`links` maps internal IDs to their corresponding URLs.
+{name}`links` maps internal IDs to their corresponding URLs.
 -/
-def xrefJson {Links} {valid} [GetElem? Links InternalId Link valid]
+public def xrefJson {Links} {valid} [GetElem? Links InternalId Link valid]
     (domains : NameMap Domain) (links : Links) : Json := Id.run do
   let mut out : Json := Json.mkObj []
   for (n, dom) in domains do
@@ -168,7 +197,7 @@ where
 /--
 An object loaded from a cross-reference database.
 -/
-structure RefObject where
+public structure RefObject where
   /-- The object's link destination. -/
   link : RemoteLink
   /-- Metadata saved for the object. -/
@@ -176,7 +205,7 @@ structure RefObject where
 deriving BEq
 
 open Format in
-instance : Repr RefObject where
+public instance : Repr RefObject where
   reprPrec v _ :=
     let {link, data} := v
     nest 2 <| group <| line.joinSep [
@@ -189,13 +218,13 @@ instance : Repr RefObject where
 /--
 Converts a reference object to the official interchange format.
 -/
-def RefObject.toJson (object : RefObject) : Json :=
+public def RefObject.toJson (object : RefObject) : Json :=
   json%{"address": $object.link.path.link, "id": $object.link.htmlId.toString, "data": $object.data}
 
 /--
 A domain loaded from a cross-reference database.
 -/
-structure RefDomain where
+public structure RefDomain where
   /--
   The domain's title field.
   -/
@@ -226,14 +255,15 @@ private unsafe def RefDomain.fastEq (x y : RefDomain) :=
 Boolean equality of reference domains.
 -/
 @[implemented_by RefDomain.fastEq]
-def RefDomain.beq := RefDomain.structEq
+private def RefDomain.beq := RefDomain.structEq
 
-instance : BEq RefDomain := ⟨RefDomain.beq⟩
+public instance : BEq RefDomain where
+  beq := private RefDomain.beq
 
 /--
 Converts a reference domain to the official interchange format.
 -/
-def RefDomain.toJson (domain : RefDomain) : Json :=
+public def RefDomain.toJson (domain : RefDomain) : Json :=
   let contents : Json := .mkObj <| domain.contents.toList.map fun (k, v) => (k, .arr <| v.map (·.toJson))
   json%{
     "title": $domain.title,
@@ -244,7 +274,7 @@ def RefDomain.toJson (domain : RefDomain) : Json :=
 /--
 Loads a set of reference domains from a cross-reference database in JSON format.
 -/
-def fromXrefJson (root : String) (json : Json) : Except String (NameMap RefDomain) := do
+public def fromXrefJson (root : String) (json : Json) : Except String (NameMap RefDomain) := do
   let json ← json.getObj?
   let mut out := {}
   let json := json.toArray
@@ -314,7 +344,7 @@ private def fetchFile (project : System.FilePath) (root : String) (file : System
 private def defaultConfigFile (project : System.FilePath) : System.FilePath := project / "verso-sources.json"
 
 /--
-Returns `true` if the user has specified a configuration file, or if they haven't and the default file exists.
+Returns {name}`true` if the user has specified a configuration file, or if they haven't and the default file exists.
 -/
 private def hasConfig (project : System.FilePath) (configFile : Option System.FilePath) : IO Bool := do
   if configFile.isSome then return true
@@ -333,7 +363,7 @@ private def getConfig (project : System.FilePath) (configFile : Option System.Fi
 /--
 Information about a remote document
 -/
-structure RemoteInfo where
+public structure RemoteInfo where
   /-- The root of the document's URLs. -/
   root : String
   /-- A short name to show in short links (e.g. "v4.20" or a package name). -/
@@ -360,21 +390,22 @@ private unsafe def RemoteInfo.fastBEq (x y : RemoteInfo) : Bool :=
 Boolean equality of information about remote documents.
 -/
 @[implemented_by RemoteInfo.fastBEq]
-def RemoteInfo.beq (x y : RemoteInfo) : Bool := RemoteInfo.structBEq x y
+private def RemoteInfo.beq (x y : RemoteInfo) : Bool := RemoteInfo.structBEq x y
 
-instance : BEq RemoteInfo := ⟨RemoteInfo.beq⟩
+public instance : BEq RemoteInfo where
+  beq := private RemoteInfo.beq
 
 /--
 All remote data that was loaded.
 -/
-structure AllRemotes where
+public structure AllRemotes where
   /-- The remote data -/
   allRemotes : HashMap String RemoteInfo := {}
 
-instance : GetElem AllRemotes String RemoteInfo (fun x y => y ∈ x.allRemotes) where
+public instance : GetElem AllRemotes String RemoteInfo (fun x y => y ∈ x.allRemotes) where
   getElem x y z := GetElem.getElem x.allRemotes y z
 
-instance : GetElem? AllRemotes String RemoteInfo (fun x y => y ∈ x.allRemotes) where
+public instance : GetElem? AllRemotes String RemoteInfo (fun x y => y ∈ x.allRemotes) where
   getElem? x y := GetElem?.getElem? x.allRemotes y
 
 private def AllRemotes.structBeq (x y : AllRemotes) : Bool :=
@@ -398,23 +429,24 @@ In compiled code, this uses pointer equality tests first, because these values a
 change during the traversal pass.
 -/
 @[implemented_by AllRemotes.fastBeq]
-def AllRemotes.beq (x y : AllRemotes) : Bool := AllRemotes.structBeq x y
+public def AllRemotes.beq (x y : AllRemotes) : Bool := AllRemotes.structBeq x y
 
 /--
-Returns an array of name-remote info pairs, in some order.b
+Returns an array of name-remote info pairs, in some order.
 -/
-def AllRemotes.toArray (all : AllRemotes) : Array (String × RemoteInfo) :=
+public def AllRemotes.toArray (all : AllRemotes) : Array (String × RemoteInfo) :=
   all.allRemotes.toArray
 
-instance : BEq AllRemotes := ⟨AllRemotes.beq⟩
+public instance : BEq AllRemotes where
+  beq := private AllRemotes.beq
 
 /--
 Updates the remote Verso data, fetching according to the configuration.
 
-`manual` should be `true` when a user is explicitly asking for a sync, not as part of something like
+{name}`manual` should be {lean}`true` when a user is explicitly asking for a sync, not as part of something like
 executing a document renderer.
 -/
-def updateRemotes (manual : Bool) (configFile : Option System.FilePath) (logVerbose : String → IO Unit) : IO AllRemotes := do
+public def updateRemotes (manual : Bool) (configFile : Option System.FilePath) (logVerbose : String → IO Unit) : IO AllRemotes := do
   let project ← findProject "."
   logVerbose s!"Loading project config. Project is '{project}'."
   if let some f := configFile then
