examples/textbook/DemoTextbook/ListSet.lean
@@ -1,0 +1,260 @@
+/-
+Copyright (c) 2025 Lean FRO LLC. All rights reserved.
+Released under Apache 2.0 license as described in the file LICENSE.
+Author: David Thrane Christiansen
+-/
+set_option doc.verso true
+
+/-!
+Here is a short demonstration of quotient types, which are used to define a type of sets that are
+represented by lists. No requirements are imposed on the type of elements, except for some operators
+that require decidable equality.
+
+The demonstration has three parts:
+ 1. First, an equivalence relation that equates any two lists with the same elements is defined.
+ 2. Next, various operations on lists are shown to preserve this relation.
+ 3. Finally, lists are quotiented by the relation, and set operations are defined using list
+    operations.
+
+In practice, this is a poor representation, because unsorted linked lists full of duplicates are not
+an efficient data structure.
+-/
+
+/-!
+# The Equivalence Relation
+-/
+
+/--
+Two lists {name}`xs` and {name}`ys` have the same contents iff any element of one is also an element
+of the other.
+-/
+@[grind]
+structure SameContents (xs ys : List α) : Prop where
+  inOne : ∀ x ∈ xs, x ∈ ys
+  inOther : ∀ y ∈ ys, y ∈ xs
+
+/--
+Every list has the same contents as itself. That is, {name}`SameContents` is reflexive.
+-/
+@[refl]
+theorem SameContents.refl (xs : List α) :
+    SameContents xs xs := by
+  constructor <;> grind
+
+/--
+{name}`SameContents` is symmetric.
+-/
+@[symm, simp, grind .]
+theorem SameContents.symm :
+    SameContents xs ys → SameContents ys xs := by
+  intro ⟨mp, mpr⟩
+  constructor <;> assumption
+
+/--
+{name}`SameContents` is transitive.
+-/
+@[simp, grind .]
+theorem SameContents.trans :
+    SameContents xs ys → SameContents ys zs →
+    SameContents xs zs := by
+  intro ⟨mp, mpr⟩ ⟨mp', mpr'⟩
+  constructor <;> grind
+
+/--
+{name}`SameContents` and {lean}`List α` form a setoid.
+-/
+def SameContents.setoid : Setoid (List α) where
+  r := SameContents
+  iseqv := ⟨SameContents.refl, SameContents.symm, SameContents.trans⟩
+
+/-!
+# List Operators and {name}`SameContents`
+
+Most list operators still make sense if we ignore the order of elements.
+-/
+
+/--
+If {name}`xs` has the same elements as the empty list, then {name}`xs` is itself empty.
+-/
+@[simp, grind .]
+theorem SameContents.empty : SameContents [] xs → xs = [] := by
+  intro ⟨mp, mpr⟩
+  cases xs
+  . rfl
+  . rename_i hd tl
+    have := mpr hd
+    simp_all
+
+/--
+If lists have the same contents, then so do the results of appending them.
+-/
+@[grind .]
+theorem SameContents.append_eq :
+    SameContents xs xs' → SameContents ys ys' →
+    SameContents (xs ++ ys) (xs' ++ ys') := by
+  induction xs <;> grind
+
+/--
+If two lists have the same contents, then removing the same elements results in them still having
+the same contents.
+-/
+@[grind .]
+theorem SameContents.filter :
+    SameContents xs ys →
+    SameContents (xs.filter p) (ys.filter p) := by
+  intro ⟨_, _⟩
+  fun_induction xs.filter p <;> grind
+
+/-!
+# The Quotient
+
+{given -show}`α : Type`
+
+Quotienting {lean}`List α` by {name}`SameContents` results in actual finite sets, because ordering
+and repetition can no longer be observed.
+-/
+
+abbrev ListSet α := Quotient (α := List α) SameContents.setoid
+
+def ListSet.mk (xs : List α) : ListSet α := Quotient.mk _ xs
+
+/-!
+## Improving Automation
+
+These helpers allow {tactic}`grind` to translate between the two representations of the setoid that
+occur in proofs, so congruence closure can propagate the needed facts. The quotient helpers cause
+the simplifier to rewrite many functions into a form where {tactic}`grind` can be used.
+-/
+
+@[grind .]
+theorem SameContents.setoid_eq_SameContents (xs ys : List α) :
+    -- This selects the desired instance over the one
+    -- in the standard library
+    let _ := setoid (α := α)
+    (xs ≈ ys) = SameContents xs ys := by
+  simp [HasEquiv.Equiv, setoid]
+
+@[grind .]
+theorem ListSet.sound {xs ys : List α} :
+    SameContents xs ys →
+    ListSet.mk xs = ListSet.mk ys := by
+  intro h; exact Quotient.sound h
+
+@[simp, grind =]
+theorem Quotient.liftOnBeta
+    {x : α} {f : α → β} {p : _} :
+    (Quotient.mk s x).liftOn f p = f x := by
+  simp [Quotient.mk]
+
+@[simp, grind =]
+theorem ListSet.liftOnBeta
+    {xs : List α} {f : List α → β} {p : _} :
+    (ListSet.mk xs).liftOn f p = f xs := by
+  simp [ListSet.mk]
+
+@[simp]
+theorem Quotient.liftOn₂beta
+    {x : α} {y : β} {f : α → β → γ} {p : _} :
+    (Quotient.mk s x).liftOn₂ (Quotient.mk s' y) f p = f x y := by
+  simp [Quotient.liftOn₂, Quotient.lift₂, Quotient.lift, Quotient.mk]
+
+@[simp]
+theorem ListSet.liftOn₂beta
+    {xs : List α} {ys : List β} {f : List α → List β → γ} {p : _} :
+    (ListSet.mk xs).liftOn₂ (ListSet.mk ys) f p = f xs ys := by
+  simp [ListSet.mk]
+
+
+/-!
+## Defining Set Operators
+
+Finally, basic set operations can be conveniently defined.
+-/
+
+/-!
+
+### Membership Test
+
+-/
+
+/--
+Checks whether {name}`x` is found in {name}`xs`
+-/
+def ListSet.contains [DecidableEq α] (xs : ListSet α) (x : α) : Bool :=
+  xs.liftOn (fun xs => x ∈ xs) (by intro _ _ ⟨_, _⟩; grind)
+
+/-!
+### Insertion
+-/
+
+/--
+Inserts {name}`x` into {name}`xs`.
+-/
+def ListSet.insert (xs : ListSet α) (x : α) : ListSet α :=
+  xs.liftOn (.mk <| x :: ·) <| by grind
+
+theorem ListSet.insert_contains
+    {_ : DecidableEq α} {xs : ListSet α} :
+    (xs.insert x).contains x = true := by
+  cases xs using Quotient.ind
+  simp [insert, contains]
+
+/-!
+### Union
+
+Union is implemented by concatenating the underlying lists. This is grossly inefficient, but easy to prove things about.
+-/
+
+def ListSet.union (xs ys : ListSet α) : ListSet α :=
+  xs.liftOn₂ ys (.mk <| · ++ ·) <| by grind
+
+/--
+The following are equivalent:
+ * $`x \in A \cup B`
+ * $`x \in A \vee x \in B`
+-/
+theorem ListSet.union_contains
+    {_ : DecidableEq α} {xs ys : ListSet α} :
+    (xs.union ys).contains x = (xs.contains x ∨ ys.contains x) := by
+  cases xs, ys using Quotient.ind₂
+  simp [union, contains]
+
+/-!
+### Membership
+
+Membership in sets is just membership in the representing list.
+-/
+
+def ListSet.Mem (xs : ListSet α) (x : α) : Prop :=
+  xs.liftOn (x ∈ ·) <| by grind
+
+instance : Membership α (ListSet α) where
+  mem := ListSet.Mem
+
+/--
+The containment test is equivalent to the membership predicate.
+-/
+theorem ListSet.mem_eq_contains
+    {_ : DecidableEq α} {xs : ListSet α} :
+    xs.contains x = (x ∈ xs) := by
+  cases xs using Quotient.ind
+  simp [contains, (· ∈ ·), Mem]
+
+/-!
+### Subtraction and Intersection
+
+Both operations are implemented using {name}`List.filter`.
+-/
+def ListSet.minus [DecidableEq α] (xs ys : ListSet α) : ListSet α :=
+  xs.liftOn₂ ys (fun xs ys => .mk <| xs.filter (· ∉ ys)) <| by grind
+
+def ListSet.intersection [DecidableEq α] (xs ys : ListSet α) : ListSet α :=
+  xs.liftOn₂ ys (fun xs ys => .mk <| xs.filter (· ∈ ys)) <| by grind
+
+theorem ListSet.intersection_commutative
+    {_ : DecidableEq α} {xs ys : ListSet α} :
+    xs.intersection ys = ys.intersection xs := by
+  induction xs, ys using Quotient.ind₂ with
+  | h xs ys =>
+    simp [intersection]
+    grind
