src/multi-verso/MultiVerso/Path.lean
@@ -3,46 +3,40 @@ Copyright (c) 2023-2025 Lean FRO LLC. All rights reserved.
 Released under Apache 2.0 license as described in the file LICENSE.
 Author: David Thrane Christiansen
 -/
+module
 
 set_option linter.missingDocs true
+set_option doc.verso true
 
 namespace Verso.Multi
 
-/-- An absolute path through the site.
+/--
 
-#[] is the root, and #[x,y,z] is s!"/{x}/{y}/{z}/". The trailing slash is important here.
+An absolute path through the site.
+
+{given (type := "String") -show}`x,y,z` {lean type:="Path"}`#[]` is the root, and {lean}`#[x,y,z]` is
+{lean}`s!"/{x}/{y}/{z}/"`. The trailing slash is important here.
 -/
-abbrev Path := Array String
+public abbrev Path := Array String
 
 namespace Path
 
 /--
 Retrieves a string that can be used as a link.
 -/
-def link (path : Path) (htmlId : Option String := none) : String :=
+public def link (path : Path) (htmlId : Option String := none) : String :=
   "/" ++ String.join (path.toList.map (· ++ "/")) ++
   (htmlId.map ("#" ++ ·)).getD ""
 
-/-- info: "/" -/
-#guard_msgs in
-#eval link #[]
-
-/-- info: "/a/b/" -/
-#guard_msgs in
-#eval link #["a", "b"]
-
-/-- info: "/a/b/#c" -/
-#guard_msgs in
-#eval link #["a", "b"] (htmlId := some "c")
 
 /--
 Make the URL relative to the path.
 
 This relies on the assumption that the path has only directory-like entries. In particular, the path
-`#["a", "b"]` is `/a/b/`. If the browser is on `/a/b/`, then `../c/` is `/a/c/`, but if it's on
+{lean}`#["a", "b"]` is `/a/b/`. If the browser is on `/a/b/`, then `../c/` is `/a/c/`, but if it's on
 `/a/b`, then `../c/` is `/c/`.
 -/
-def relativize (path : Path) (url : String) : String := Id.run do
+public def relativize (path : Path) (url : String) : String := Id.run do
   if "/".isPrefixOf url then
     let mut path := path.toSubarray
     let mut url := url.toSubstring.drop 1
@@ -54,69 +48,5 @@ def relativize (path : Path) (url : String) : String := Id.run do
       else break
     String.join (List.replicate path.size "../") ++ url.toString
   else url
-
-/- Tests for relativization. -/
-
-/-- info: "a/b/c/" -/
-#guard_msgs in
-#eval Path.relativize #[] "/a/b/c/"
-/-- info: "a/b/c/#foo" -/
-#guard_msgs in
-#eval Path.relativize #[] "/a/b/c/#foo"
-/-- info: "a/b/c#foo" -/
-#guard_msgs in
-#eval Path.relativize #[] "/a/b/c#foo"
-
-/-- info: "b/c/" -/
-#guard_msgs in
-#eval Path.relativize #["a"] "/a/b/c/"
-/-- info: "b/c/#foo" -/
-#guard_msgs in
-#eval Path.relativize #["a"] "/a/b/c/#foo"
-/-- info: "b/c#foo" -/
-#guard_msgs in
-#eval Path.relativize #["a"] "/a/b/c#foo"
-
-/-- info: "c/" -/
-#guard_msgs in
-#eval Path.relativize #["a", "b"] "/a/b/c/"
-/-- info: "c/#foo" -/
-#guard_msgs in
-#eval Path.relativize #["a", "b"] "/a/b/c/#foo"
-/-- info: "c#foo" -/
-#guard_msgs in
-#eval Path.relativize #["a", "b"] "/a/b/c#foo"
-
-/-- info: "../../aa/b/c#foo" -/
-#guard_msgs in
-#eval Path.relativize #["a", "b"] "/aa/b/c#foo"
-
-/-- info: "../" -/
-#guard_msgs in
-#eval Path.relativize #["a", "b", "c", "d"] "/a/b/c/"
-/-- info: "../../c" -/
-#guard_msgs in
-#eval Path.relativize #["a", "b", "c", "d"] "/a/b/c"
-
-/-- info: "../#foo" -/
-#guard_msgs in
-#eval Path.relativize #["a", "b", "c", "d"] "/a/b/c/#foo"
-/-- info: "../../" -/
-#guard_msgs in
-#eval Path.relativize #["a", "b", "c", "d", "e"] "/a/b/c/"
-/-- info: "../../#foo" -/
-#guard_msgs in
-#eval Path.relativize #["a", "b", "c", "d", "e"] "/a/b/c/#foo"
-/-- info: "../../../c#foo" -/
-#guard_msgs in
-#eval Path.relativize #["a", "b", "c", "d", "e"] "/a/b/c#foo"
-
-/-- info: "../../../c" -/
-#guard_msgs in
-#eval Path.relativize #["a", "b", "c", "d", "e"] "/a/b/c"
-
-/-- info: "" -/
-#guard_msgs in
-#eval Path.relativize #[] "/"
 
 end Path
