src/verso-blog/VersoBlog/LiterateModuleDocs.lean
@@ -1,0 +1,148 @@
+/-
+Copyright (c) 2025 Lean FRO LLC. All rights reserved.
+Released under Apache 2.0 license as described in the file LICENSE.
+Author: David Thrane Christiansen
+-/
+import SubVerso.Helper
+import SubVerso.Module
+import VersoBlog.Basic
+import VersoBlog.LiterateLeanPage.Options
+import MD4Lean
+import VersoLiterate
+
+set_option doc.verso true
+
+open Verso Doc
+open Lean
+
+open SubVerso.Highlighting
+open SubVerso.Helper
+open SubVerso.Module
+open Verso.Doc.Concrete (stringToInlines)
+
+namespace Verso.Genre.Blog.Literate
+
+open VersoLiterate
+
+instance [bg : BlogGenre g] : LoadLiterate g where
+  inline goI
+    | .highlighted hl, content =>
+      .other (bg.inline_eq ▸ .highlightedCode { contextName := `lean } hl) <| content.map goI
+    | .data .., xs => .concat <| xs.map goI
+  block _goI goB
+    | .highlighted hl, content =>
+      .other (bg.block_eq ▸ .highlightedCode { contextName := `lean } hl) <| content.map goB
+    | .data .., xs => .concat <| xs.map goB
+
+  docstring indent declName? xs := .other (bg.block_eq ▸ .docstring indent declName?) xs
+
+  docstringPart lvl title content :=
+    .other (bg.block_eq ▸ .docstringSection lvl) <|
+      #[.para title] ++ content
+
+
+section
+variable [Monad m] [MonadError m] [MonadQuotation m]
+
+
+open Verso Doc in
+open Lean Elab Command Term in
+open PartElabM in
+def elabFromModuleDocs (x : Ident) (path : StrLit) (mod : Ident) (title : StrLit) (genre : Term) (metadata? : Option Term) : CommandElabM Unit :=
+  withTraceNode `verso.blog.literate (fun _ => pure m!"Literate '{title.getString}'") do
+
+  let titleParts ← stringToInlines title
+  let titleString := inlinesToString (← getEnv) titleParts
+  let initState : PartElabM.State := .init (.node .none nullKind titleParts)
+
+
+  let g ← runTermElabM fun _ => Term.elabTerm genre (some (.const ``Doc.Genre []))
+
+  let (titleTerm, _st) ← liftTermElabM <| DocElabM.run genre g {} initState <| do
+    titleParts.mapM (elabInline ⟨·⟩)
+
+  let modJson ← withTraceNode `verso.blog.literate.loadMod (fun _ => pure m!"Loading '{mod}' in '{path}'") <|
+    loadModuleJson path.getString mod.getId.toString
+
+  let jsonName ← runTermElabM fun _ => do
+    let name ← mkFreshUserName (x.getId ++ `json)
+    addAndCompile <| .defnDecl {
+      name, levelParams := [], type := mkConst ``String, value := mkStrLit modJson,
+      hints := .regular 0, safety := .safe
+    }
+    pure name
+
+  let mod ← runTermElabM fun _ => do
+    let name ← mkFreshUserName (x.getId ++ `getPart)
+    let title ← titleTerm.mapM (elabTerm · (some (.app (mkConst ``Verso.Doc.Inline) g)))
+    let title ← Meta.mkArrayLit (.app (mkConst ``Verso.Doc.Inline) g) title.toList
+    withOptions (Compiler.LCNF.compiler.extract_closed.set · false) do
+      addAndCompile <| .defnDecl {
+        name, levelParams := [], type := .app (mkConst ``Verso.Doc.Part) g,
+        value := ← Meta.mkAppM ``modToPage! #[
+          ← Meta.mkAppM ``VersoLiterate.loadJsonString! #[mkConst jsonName, mkStrLit s!"JSON for {x.getId}"],
+          title,
+          mkStrLit titleString
+        ],
+        hints := .regular 0, safety := .safe
+      }
+    pure name
+
+  let metadata ← if let some m := metadata? then `(some $m) else `(none)
+  elabCommand <| ← `(command|def $x : Part $genre := {$(mkIdent mod) with metadata := $metadata})
+
+
+end
+
+end Literate
+open Literate
+
+open Lean.Parser (sepByIndent)
+open Lean.Parser.Term
+open Verso.Doc.Concrete
+
+open Lean.Parser.Tactic
+
+/--
+Creates a post from a literate Lean module with Verso-based module docstrings in it. Markdown module
+docstrings are supported, but no attempt is made to elaborate included code.
+
+Specifically, `literate_page POST from MOD in DIR as TITLE` defines a post {lit}`POST` by elaborating the
+module {lit}`MOD` in the project directory {lit}`DIR` with title {lit}`TITLE`.
+
+{lit}`DIR` should be a project directory that contains a toolchain file and a Lake configuration
+(`lakefile.toml` or `lakefile.lean`), which should depend on the same version of Verso that this
+website is using.
+-/
+syntax "literate_page " ident optConfig " from " ident " in " str " as " str (" with " term)? : command
+/--
+Creates a post from a literate Lean module with Verso-based module docstrings in it. Markdown module
+docstrings are supported, but no attempt is made to elaborate included code.
+
+Specifically, `literate_post POST from MOD in DIR as TITLE` defines a post {lit}`POST` by elaborating the
+module {lit}`MOD` in the project directory {lit}`DIR` with title {lit}`TITLE`.
+
+{lit}`DIR` should be a project directory that contains a toolchain file and a Lake configuration
+(`lakefile.toml` or `lakefile.lean`), which should depend on the same version of Verso that this
+website is using.
+-/
+syntax "literate_post " ident optConfig " from " ident " in " str " as " str (" with " term)? : command
+
+open Verso Doc in
+open Lean Elab Command in
+elab_rules : command
+  | `(literate_page $x from $mod in $path as $title $[with $metadata]?) => do
+
+    withScope (fun sc => {sc with opts := Elab.async.set sc.opts false}) do
+      let genre ← `(Page)
+      elabFromModuleDocs x path mod title genre metadata
+
+
+open Verso Doc in
+open Lean Elab Command in
+elab_rules : command
+  | `(literate_post $x from $mod in $path as $title $[with $metadata]?) => do
+
+    withScope (fun sc => {sc with opts := Elab.async.set sc.opts false}) do
+      let genre ← `(Post)
+      elabFromModuleDocs x path mod title genre metadata
