src/verso-literate/VersoLiterate/Module.lean
@@ -1,0 +1,94 @@
+/-
+Copyright (c) 2025 Lean FRO LLC. All rights reserved.
+Released under Apache 2.0 license as described in the file LICENSE.
+Author: David Thrane Christiansen
+-/
+import Verso.BEq
+import VersoLiterate.Exported
+import Verso.Doc
+
+namespace VersoLiterate
+open Lean
+open Verso.Doc
+
+def loadJsonString (jsonString : String) (blame := "JSON string") : Except String LitMod := do
+  let json ← Lean.Json.parse jsonString |>.mapError (s!"Error parsing {blame}: {·}")
+  let name ← json.getObjValAs? String "module" |>.mapError (s!"Error decoding module name in {blame}: {·}")
+  let itemsJson ← json.getObjVal? "items" |>.mapError (s!"Error decoding items in {blame}: {·}")
+  let eItems ← FromJson.fromJson? (α := VersoLiterate.ExportedModuleItems) itemsJson |>.mapError (s!"Error decoding {blame}: {·}")
+  let items ← eItems.toModuleItems
+  pure { name := name.toName, contents := items }
+
+def loadJsonString! (jsonString : String) (blame := "JSON string") : LitMod :=
+  match loadJsonString jsonString blame with
+  | .error e => panic! e
+  | .ok v => v
+
+def load (jsonFile : System.FilePath) : IO LitMod := do
+  let json ← IO.FS.readFile jsonFile
+  match loadJsonString json (blame := jsonFile.toString) with
+  | .error e => throw <| .userError e
+  | .ok v => pure v
+
+def modToPage! [LoadLiterate g] (mod : LitMod) (title : Array (Inline g)) (titleString : String) : Part g :=
+  match modToPage mod title titleString with
+  | .error e => panic! s!"Couldn't load {titleString}: {e}"
+  | .ok v => v
+
+open System in
+def loadModuleJson
+    (leanProject : FilePath) (mod : String)
+    (overrideToolchain : Option String := none) : IO String := do
+
+  let projectDir := ((← IO.currentDir) / leanProject).normalize
+
+  -- Validate that the path is really a Lean project
+  let lakefile := projectDir / "lakefile.lean"
+  let lakefile' := projectDir / "lakefile.toml"
+  if !(← lakefile.pathExists) && !(← lakefile'.pathExists) then
+    throw <| .userError s!"Neither {lakefile} nor {lakefile'} exist, couldn't load project"
+  let toolchain ← match overrideToolchain with
+    | none =>
+      let toolchainfile := projectDir / "lean-toolchain"
+      if !(← toolchainfile.pathExists) then
+        throw <| .userError s!"File {toolchainfile} doesn't exist, couldn't load project"
+      pure (← IO.FS.readFile toolchainfile).trim
+    | some override => pure override
+
+  -- Kludge: remove variables introduced by Lake. Clearing out DYLD_LIBRARY_PATH and
+  -- LD_LIBRARY_PATH is useful so the version selected by Elan doesn't get the wrong shared
+  -- libraries.
+  let lakeVars :=
+    #["LAKE", "LAKE_HOME", "LAKE_PKG_URL_MAP",
+      "LEAN_SYSROOT", "LEAN_AR", "LEAN_PATH", "LEAN_SRC_PATH",
+      "LEAN_GITHASH",
+      "ELAN_TOOLCHAIN", "DYLD_LIBRARY_PATH", "LD_LIBRARY_PATH"]
+  let cmd := "elan"
+  let args := #["run", "--install", toolchain, "lake", "query", s!"+{mod}:literate"]
+  let res ← IO.Process.output {
+    cmd, args, cwd := projectDir
+    -- Unset Lake's environment variables
+    env := lakeVars.map (·, none)
+  }
+  if res.exitCode != 0 then reportFail projectDir cmd args res
+  if let some f := res.stdout.split (· == '\n') |>.find? (!·.isEmpty) then
+    IO.FS.readFile f
+  else throw <| .userError s!"No result returned from build of {mod}"
+
+where
+  decorateOut (name : String) (out : String) : String :=
+    if out.isEmpty then "" else s!"\n{name}:\n{out}\n"
+  reportFail {α} (projectDir : FilePath) (cmd : String) (args : Array String) (res : IO.Process.Output) : IO α := do
+    IO.eprintln <|
+      "Build process failed." ++
+      "\nCWD: " ++ projectDir.toString ++
+      "\nCommand: " ++ cmd ++
+      "\nArgs: " ++ repr args ++
+      "\nExit code: " ++ toString res.exitCode ++
+      "\nstdout: " ++ res.stdout ++
+      "\nstderr: " ++ res.stderr
+
+    throw <| .userError <|
+      "Build process failed." ++
+      decorateOut "stdout" res.stdout ++
+      decorateOut "stderr" res.stderr
