src/verso-manual/VersoManual/Literate.lean
@@ -1,0 +1,139 @@
+/-
+Copyright (c) 2025 Lean FRO LLC. All rights reserved.
+Released under Apache 2.0 license as described in the file LICENSE.
+Author: David Thrane Christiansen
+-/
+import VersoManual.Basic
+import VersoManual.ExternalLean
+import VersoLiterate
+import Lean.Data.Json
+
+namespace Verso.Genre.Manual
+
+open VersoLiterate
+open Verso.Code.External
+open Verso.Output Html
+open Verso.Doc.Html
+open Lean
+
+block_extension Block.literateDocstring where
+  traverse _ _ _ _ := pure none
+  toHtml := some fun _goI goB _id _data contents => do
+    pure {{<div class="literate-docstring">{{← contents.mapM goB}}</div>}}
+  toTeX := none
+
+block_extension Block.literateDocstringPart (level : Nat) where
+  data := level
+  traverse _ _ _ _ := pure none
+  toHtml := some fun goI goB _id data contents => do
+    let .ok (level : Nat) := FromJson.fromJson? data
+      | HtmlT.logError s!"Couldn't decode nesting level from {data.compress}"
+        pure .empty
+    let title : Html ←
+      if let some title := contents[0]? then
+        if let .para xs := title then
+          xs.mapM goI
+        else
+          HtmlT.logError s!"Expected a paragraph at the beginning of a docstring section"
+          pure .empty
+      else
+        HtmlT.logError s!"Expected a block at the beginning of a docstring section"
+        pure .empty
+    let contents := contents.extract 1
+    pure {{
+      <section>
+        {{.tag s!"h{level + 1}" #[] title}}
+        {{← contents.mapM goB}}
+      </section>
+    }}
+  toTeX := none
+
+
+instance : LoadLiterate Manual where
+  inline goI
+    | .highlighted hl, _ => ExternalCode.leanInline hl {}
+    | .data .., content => .concat <| content.map goI
+
+  block _goI goB
+    | .highlighted hl, _ => ExternalCode.leanBlock hl {}
+    | .data .., content => .concat <| content.map goB
+
+  docstring _indent _declName? content := .other Block.literateDocstring content
+
+  docstringPart lvl title contents := .other (Block.literateDocstringPart lvl) (#[.para title] ++ contents)
+
+open Lean.Doc.Syntax
+open Verso.Doc Elab Concrete
+open Lean.Elab Command Term
+open PartElabM
+def getModuleWithDocs (path : StrLit) (mod : Ident) (title : StrLit) : PartElabM Name :=
+  withTraceNode `verso.blog.literate (fun _ => pure m!"Literate '{title.getString}'") do
+
+  let titleParts ← stringToInlines title
+  let titleString := inlinesToString (← getEnv) titleParts
+  let initState : PartElabM.State := .init (.node .none nullKind titleParts)
+
+  let genre ← ``(Manual)
+  let g := Expr.const ``Manual []
+
+  let (titleTerm, _st) ← DocElabM.run genre g {} initState <| do
+    titleParts.mapM (elabInline ⟨·⟩)
+
+  let modJson ← withTraceNode `verso.blog.literate.loadMod (fun _ => pure m!"Loading '{mod}' in '{path}'") <|
+    loadModuleJson path.getString mod.getId.toString
+
+  let jsonName ← do
+    let name ← mkFreshUserName (mod.getId ++ `json)
+    addAndCompile <| .defnDecl {
+      name, levelParams := [], type := mkConst ``String, value := mkStrLit modJson,
+      hints := .regular 0, safety := .safe
+    }
+    pure name
+
+  let mod ← do
+    let name ← mkFreshUserName (mod.getId ++ `getPart)
+    let title ← titleTerm.mapM (elabTerm · (some (.app (mkConst ``Verso.Doc.Inline) g)))
+    let title ← Meta.mkArrayLit (.app (mkConst ``Verso.Doc.Inline) g) title.toList
+    withOptions (Compiler.LCNF.compiler.extract_closed.set · false) do
+      addAndCompile <| .defnDecl {
+        name, levelParams := [], type := .app (mkConst ``Verso.Doc.Part) g,
+        value := ← Meta.mkAppM ``modToPage! #[
+          ← Meta.mkAppM ``VersoLiterate.loadJsonString! #[mkConst jsonName, mkStrLit s!"JSON for {mod.getId}"],
+          title,
+          mkStrLit titleString
+        ],
+        hints := .regular 0, safety := .safe
+      }
+    pure name
+  return mod
+
+section
+open ArgParse
+
+variable [Monad m] [MonadError m] [MonadLiftT CoreM m]
+
+structure IncludeLiterateConfig where
+  path : StrLit
+  level : Option NumLit
+  modName : Ident
+  title : StrLit
+
+instance : FromArgs IncludeLiterateConfig m where
+  fromArgs :=
+    IncludeLiterateConfig.mk <$> .positional' `path  <*> .named' `level true <*> .positional' `name <*> .positional' `title
+
+
+@[part_command Lean.Doc.Syntax.command]
+def includeLiterateSection : PartCommand
+  | `(block|command{includeLiterate $args* }) => do
+    let {path, level, modName, title} ← parseThe IncludeLiterateConfig (← parseArgs args)
+    let ref ← getRef
+    if let some lvl := level then
+      let name ← getModuleWithDocs path modName title
+      closePartsUntil lvl.getNat ref.getHeadInfo.getPos!
+      addPart <| .included (mkIdentFrom modName name)
+    else
+      let name ← getModuleWithDocs path modName title
+      addPart <| .included (mkIdentFrom modName name)
+
+  | _ => (Lean.Elab.throwUnsupportedSyntax : PartElabM Unit)
