src/verso-util/VersoUtil/BinFiles.lean
@@ -3,20 +3,20 @@ Copyright (c) 2025 Lean FRO LLC. All rights reserved.
 Released under Apache 2.0 license as described in the file LICENSE.
 Author: David Thrane Christiansen
 -/
-import Lean.Elab.Eval
-import Lean.Elab.Term
-import VersoUtil.BinFiles.Z85
+module
+
+meta import Lean.Elab.Eval
+public meta import Lean.Elab.Term
+-- Both imports are needed: the `meta` import is for encoding the files at compile time, which emits
+-- a call to the non-`meta` decoder at run time. This is because it's much easier to move strings
+-- across phases than byte arrays.
+meta import VersoUtil.BinFiles.Z85
+public import VersoUtil.BinFiles.Z85
 
 open Lean Elab Term
 open Lean Environment
 
 namespace Verso.BinFiles
-
-private unsafe def evalFilePathUnsafe (stx : Syntax) : TermElabM System.FilePath :=
-  evalTerm System.FilePath (Lean.mkConst ``System.FilePath) stx
-
-@[implemented_by evalFilePathUnsafe]
-private opaque evalFilePath (stx : Syntax) : TermElabM System.FilePath
 
 /--
 Includes a binary file in the Lean module. The source path is given relative to the current file.
@@ -25,7 +25,7 @@ Internally, the file's contents are represented using a string literal in the Z8
 similar to Base64 but more efficient.
 -/
 elab "include_bin " path:str : term => do
-  let path ← evalFilePath path
+  let path : System.FilePath := path.getString
   let ctx ← readThe Lean.Core.Context
   let srcPath := System.FilePath.mk ctx.fileName
   let some srcDir := srcPath.parent
@@ -34,7 +34,7 @@ elab "include_bin " path:str : term => do
   let contents ← IO.FS.readBinFile path
   return mkApp2 (.const ``Z85.decode []) (mkStrLit (Z85.encode contents)) (toExpr contents.size)
 
-private partial def binFiles (base : System.FilePath) (path : System.FilePath) : IO (Array (System.FilePath × Expr)) :=
+private meta partial def binFiles (base : System.FilePath) (path : System.FilePath) : IO (Array (System.FilePath × Expr)) :=
   (·.snd) <$> StateT.run (go base path) #[]
 where
   go (base path : System.FilePath) : StateT (Array _) IO Unit := do
@@ -62,7 +62,7 @@ Internally, the files' contents are represented using string literals in the Z85
 similar to Base64 but more efficient.
 -/
 elab "include_bin_dir " path:str : term => do
-  let path ← evalFilePath path
+  let path : System.FilePath := path.getString
   let ctx ← readThe Lean.Core.Context
   let srcPath := System.FilePath.mk ctx.fileName
   let some srcDir := srcPath.parent
