src/verso/Verso/Doc/PointOfInterest.lean
@@ -3,22 +3,21 @@ Copyright (c) 2024 Lean FRO LLC. All rights reserved.
 Released under Apache 2.0 license as described in the file LICENSE.
 Author: David Thrane Christiansen
 -/
-
-import Lean.Server.CodeActions
+module
+public import Lean.Server.CodeActions
 
 namespace Verso.Doc
 
 open Lean Elab Server RequestM
 
-structure PointOfInterest where
+public structure PointOfInterest where
   title : String
   selectionRange : Option String.Range := none
   kind : Lean.Lsp.SymbolKind := .constant
   detail? : Option String
-
 deriving TypeName
 
-def PointOfInterest.save [Monad m] [MonadInfoTree m] (stx : Syntax) (title : String)
+public def PointOfInterest.save [Monad m] [MonadInfoTree m] (stx : Syntax) (title : String)
     (selectionRange : Syntax := stx)
     (kind : Lean.Lsp.SymbolKind := .constant)
     (detail? : Option String := none) : m Unit := do
