src/verso/Verso/Hint.lean
@@ -3,30 +3,51 @@ Copyright (c) 2025 Lean FRO LLC. All rights reserved.
 Released under Apache 2.0 license as described in the file LICENSE.
 Author: David Thrane Christiansen
 -/
+module
+public import Lean.Message
+public import Lean.Meta.Hint
 
-import Lean.Message
-import Lean.Meta.Hint
+
+set_option doc.verso true
+set_option pp.rawOnError true
 
 open Lean Meta Hint
 
 namespace Verso
 
-/-
+/--
 Creates a hint message with associated code action suggestions at a specified location.
 
 The arguments are as follows:
-* `ref`: the syntax location for the code action suggestions. Will be overridden by the `span?`
-  field on any suggestions that specify it.
-* `hint`: the main message of the hint, which precedes its code action suggestions.
-* `suggestions`: the suggestions to display.
-* `codeActionPrefix?`: if specified, text to display in place of "Try this: " in the code action
-  label
-* `forceList`: if `true`, suggestions will be displayed as a bulleted list even if there is only
-  one.
+
+: {name}`ref`
+
+  the syntax location for the code action suggestions. Will be overridden by the
+  {name}`Suggestion.span?` field on any suggestions that specify it.
+
+: {name}`hint`
+
+  the main message of the hint, which precedes its code action suggestions.
+
+: {name}`suggestions`
+
+  the suggestions to display.
+
+: {name}`codeActionPrefix?`
+
+  if specified, text to display in place of "Try this: " in the code action label
+
+: {name}`forceList`
+
+  if {name}`true`, suggestions will be displayed as a bulleted list even if there
+  is only one.
 -/
-def hintAt (ref : Syntax) (hint : MessageData) (suggestions : Array Suggestion)
+public def hintAt (ref : Syntax) (hint : MessageData) (suggestions : Array Suggestion)
     (codeActionPrefix? : Option String := none)
     (forceList : Bool := false) :
     CoreM MessageData :=
   -- The @ guards against upstream signature changes going unnoticed
-  @MessageData.hint hint suggestions (ref? := some ref) (codeActionPrefix? := codeActionPrefix?) (forceList := forceList)
+  @MessageData.hint hint suggestions
+    (ref? := some ref)
+    (codeActionPrefix? := codeActionPrefix?)
+    (forceList := forceList)
