src/verso/Verso/Output/Html/ElasticLunr.lean
@@ -3,6 +3,8 @@ Copyright (c) 2025 Lean FRO LLC. All rights reserved.
 Released under Apache 2.0 license as described in the file LICENSE.
 Author: David Thrane Christiansen
 -/
+module
+meta import Init
 
 set_option linter.missingDocs true
 
@@ -11,11 +13,11 @@ namespace Verso.Output.Html
 /--
 The minified elasticlunr JS file's contents.
 -/
-def elasticlunr.min.js : String :=
+public def elasticlunr.min.js : String :=
   include_str "../../../../../vendored-js/elasticlunr/elasticlunr.min.js"
 
 /--
 The complete elasticlunr JS file's contents.
 -/
-def elasticlunr.js : String :=
+public def elasticlunr.js : String :=
   include_str "../../../../../vendored-js/elasticlunr/elasticlunr.js"
